Splitting pattern match on bitvectors

theories/Shallow/Executor.v
@@ -46,6 +46,7 @@ From stdpp Require base list option.
 Import ctx.notations.
 Import env.notations.
 Import ListNotations.
+Import SigTNotations.
 
 Set Implicit Arguments.
 
@@ -836,10 +837,10 @@ Module Type ShallowExecOn
 
       Definition demonic_match_bvec {A n} {Γ1 Γ2} :
         Val (ty.bvec n) -> (bv n -> CHeapSpecM Γ1 Γ2 A) -> CHeapSpecM Γ1 Γ2 A :=
-        fun v POST =>
+        fun v k =>
           u <- demonic_finite (bv n);;
           assume_formula (v = u);;
-          POST u.
+          k u.
       #[global] Arguments demonic_match_bvec : simpl never.
 
       Lemma wp_demonic_match_bvec {A n Γ1 Γ2} (v : Val (ty.bvec n)) (k : bv n -> CHeapSpecM Γ1 Γ2 A) :
@@ -853,6 +854,31 @@ Module Type ShallowExecOn
         apply H; auto.
         rewrite <- base.elem_of_list_In.
         apply finite.elem_of_enum.
+      Qed.
+
+      Definition demonic_match_bvec_split {A m n} {Γ1 Γ2} :
+        Val (ty.bvec (m + n)) ->
+        (bv m -> bv n -> CHeapSpecM Γ1 Γ2 A) -> CHeapSpecM Γ1 Γ2 A :=
+        fun v k =>
+          v1 <- demonic (ty.bvec m) ;;
+          v2 <- demonic (ty.bvec n) ;;
+          assume_formula (bv.app v1 v2 = v) ;;
+          k v1 v2.
+      #[global] Arguments demonic_match_bvec_split : simpl never.
+
+      Lemma wp_demonic_match_bvec_split {A m n Γ1 Γ2}
+        (v : Val (ty.bvec (m + n))) (k : bv m -> bv n -> CHeapSpecM Γ1 Γ2 A) :
+        forall POST δ h,
+          demonic_match_bvec_split v k POST δ h <->
+          match bv.appView m n v with
+          | bv.isapp xs ys => k xs ys POST δ h
+          end.
+      Proof.
+        intros POST δ h.
+        cbv [demonic_match_bvec_split bind demonic bind_right
+           assume_formula lift_purem CPureSpecM.assume_formula].
+        destruct (bv.appView m n v) as [v1 v2].
+        split; [auto|]. now intros ? * [-> ->]%bv.app_inj.
       Qed.
 
     End PatternMatching.
@@ -1127,6 +1153,14 @@ Module Type ShallowExecOn
               demonic_match_bvec
                 v
                 (fun u => exec_aux (rhs u))
+            | stm_match_bvec_split m n e xl xr rhs =>
+              v <- eval_exp e ;;
+              demonic_match_bvec_split
+                v
+                (fun vl vr =>
+                   pushspops
+                     [kv (xl∷ty.bvec m; vl); (xr∷ty.bvec n; vr)]
+                     (exec_aux rhs))
             | stm_bind s k =>
               v <- exec_aux s ;;
               exec_aux (k v)
